Bring in the rest of the loops into kremlib/C.Loops.fst

kremlib/C.Loops.fst
@@ -1,8 +1,7 @@
-module C.Loops
-
-(* This modules exposes a series of combinators; they are modeled using
+(** This modules exposes a series of combinators; they are modeled using
  * higher-order functions and specifications, and extracted, using a
  * meta-theoretic argument, to actual C loops. *)
+module C.Loops
 
 open FStar.ST
 open FStar.Buffer
@@ -13,12 +12,25 @@ module UInt32 = FStar.UInt32
 
 #set-options "--initial_fuel 0 --max_fuel 0 --z3rlimit 20"
 
-(* To be extracted as:
-  {
-    int i = <start>;
-    for (; i != <finish>; ++i) <f>;
-  }
-  // i need not be in scope after the loop
+(** The functions in this module use the following convention:
+ *  - the first arguments are buffers;
+ *  - the destination buffer comes first, followed by the input buffer (as in
+ *    C's memcpy)
+ *  - each buffer is followed by its length; if several buffers share the same
+ *    length, there is a single length argument after the buffers
+ *  - the function-specific arguments come next (e.g. the number of times one
+ *    may want to call the function in [repeat])
+ *  - the second to last argument is the loop invariant (which may have
+ *    dependencies on all the parameters before)
+ *  - the last argument is the loop body (that will depend on the invariant, and
+ *    possibly all the other parameters before. *)
+
+
+(* Generic-purpose for-loop combinators ***************************************)
+
+(* Currently extracting as:
+    for (int i = <start>; i != <finish>; ++i)
+      <f> i;
 *)
 val for:
   start:UInt32.t ->
@@ -39,11 +51,8 @@ let rec for start finish inv f =
   end
 
 (* To be extracted as:
-  {
-    int i = <start>;
-    for (; i != <finish>; --i) <f>;
-  }
-  // i need not be in scope after the loop
+    for (int i = <start>; i != <finish>; --i)
+      <f> i;
 *)
 val reverse_for:
   start:UInt32.t ->
@@ -67,7 +76,7 @@ let rec reverse_for start finish inv f =
     int i = <start>;
     bool b = false;
     for (; (!b) && (i != <end>); ++i) {
-      b = <f>;
+      b = <f> i;
     }
     // i and b must be in scope after the loop
 *)
@@ -94,9 +103,9 @@ let rec interruptible_for start finish inv f =
     int i = <start>;
     bool b = false;
     for (; (!b) && (i != <end>); --i) {
-      b = <f>;
+      b = <f> i;
     }
-    // i and b must be in scope after the loop    
+    // i and b must be in scope after the loop
 *)
 val interruptible_reverse_for:
   start:UInt32.t ->
@@ -118,11 +127,13 @@ let rec interruptible_reverse_for start finish inv f =
     else interruptible_reverse_for start' finish inv f
 
 
+(* Mapping the contents of a buffer into another ******************************)
+
 val seq_map:
   #a:Type -> #b:Type ->
   f:(a -> Tot b) ->
   s:Seq.seq a ->
-  Tot (s':Seq.seq b{Seq.length s = Seq.length s' /\ 
+  Tot (s':Seq.seq b{Seq.length s = Seq.length s' /\
     (forall (i:nat). {:pattern (Seq.index s' i)} i < Seq.length s' ==> Seq.index s' i == f (Seq.index s i))})
     (decreases (Seq.length s))
 let rec seq_map #a #b f s =
@@ -132,14 +143,18 @@ let rec seq_map #a #b f s =
     let s' = Seq.cons (f (Seq.head s)) (seq_map f (Seq.tail s)) in
     s'
 
-(* To be substituted with its definition *)
+
+(** Extracts as:
+ * for (int i = 0; i < <l>; ++i)
+ *   out[i] = <f>(in[i]);
+ *)
 inline_for_extraction
 val map:
   #a:Type0 -> #b:Type0 ->
-  f:(a -> Tot b) ->
   output: buffer b ->
   input: buffer a{disjoint input output} ->
   l: UInt32.t{ UInt32.v l = Buffer.length output /\ UInt32.v l = Buffer.length input } ->
+  f:(a -> Tot b) ->
   Stack unit
     (requires (fun h -> live h input /\ live h output ))
     (ensures (fun h_1 r h_2 -> modifies_1 output h_1 h_2 /\ live h_2 input /\ live h_1 input /\ live h_2 output
@@ -148,7 +163,7 @@ val map:
          let s2 = as_seq h_2 output in
          s2 == seq_map f s1) ))
 inline_for_extraction
-let map #a #b f output input l =
+let map #a #b output input l f =
   let h0 = ST.get() in
   let inv (h1: HS.mem) (i: nat): Type0 =
     live h1 output /\ live h1 input /\ modifies_1 output h0 h1 /\ i <= UInt32.v l
@@ -164,3 +179,183 @@ let map #a #b f output input l =
   for 0ul l inv f';
   let h1 = ST.get() in
   Seq.lemma_eq_intro (as_seq h1 output) (seq_map f (as_seq h0 input))
+
+
+val seq_map2:
+  #a:Type -> #b:Type -> #c:Type ->
+  f:(a -> b -> Tot c) ->
+  s:Seq.seq a -> s':Seq.seq b{Seq.length s = Seq.length s'} ->
+  Tot (s'':Seq.seq c{Seq.length s = Seq.length s'' /\
+    (forall (i:nat). {:pattern (Seq.index s'' i)} i < Seq.length s'' ==> Seq.index s'' i == f (Seq.index s i) (Seq.index s' i))})
+    (decreases (Seq.length s))
+let rec seq_map2 #a #b #c f s s' =
+  if Seq.length s = 0 then Seq.createEmpty
+  else
+    let s'' = Seq.cons (f (Seq.head s) (Seq.head s')) (seq_map2 f (Seq.tail s) (Seq.tail s')) in
+    s''
+
+
+(** Extracts as:
+ * for (int i = 0; i < <l>; ++i)
+ *   out[i] = <f>(in1[i], in2[i]);
+ *)
+val map2:
+  #a:Type0 -> #b:Type0 -> #c:Type0 ->
+  output: buffer c ->
+  in1: buffer a{disjoint output in1} -> in2: buffer b{disjoint output in2} ->
+  l: UInt32.t{ UInt32.v l = Buffer.length output /\ UInt32.v l = Buffer.length in1
+     /\ UInt32.v l = Buffer.length in2 } ->
+  f:(a -> b -> Tot c) ->
+  Stack unit
+    (requires (fun h -> live h in1 /\ live h in2 /\ live h output ))
+    (ensures (fun h_1 r h_2 -> modifies_1 output h_1 h_2 /\ live h_2 in1 /\ live h_2 in2
+      /\ live h_1 in1 /\ live h_1 in2 /\ live h_2 output
+      /\ (let s1 = as_seq h_1 in1 in
+         let s2 = as_seq h_1 in2 in
+         let s = as_seq h_2 output in
+         s == seq_map2 f s1 s2) ))
+let map2 #a #b #c output in1 in2 l f =
+  let h0 = ST.get() in
+  let inv (h1: HS.mem) (i: nat): Type0 =
+    live h1 output /\ live h1 in1 /\ live h1 in2 /\ modifies_1 output h0 h1 /\ i <= UInt32.v l
+    /\ (forall (j:nat). {:pattern (get h1 output j)} (j >= i /\ j < UInt32.v l) ==> get h1 output j == get h0 output j)
+    /\ (forall (j:nat). {:pattern (get h1 output j)} j < i ==> get h1 output j == f (get h0 in1 j) (get h0 in2 j))
+  in
+  let f' (i:UInt32.t{ UInt32.( 0 <= v i /\ v i < v l ) }): Stack unit
+    (requires (fun h -> inv h (UInt32.v i)))
+    (ensures (fun h_1 _ h_2 -> UInt32.(inv h_2 (v i + 1))))
+  =
+    output.(i) <- f (in1.(i)) (in2.(i))
+  in
+  for 0ul l inv f';
+  let h1 = ST.get() in
+  Seq.lemma_eq_intro (as_seq h1 output) (seq_map2 f (as_seq h0 in1) (as_seq h0 in2))
+
+
+(** Extracts as:
+ * for (int i = 0; i < <l>; ++i)
+ *   b[i] = <f>(b[i]);
+ *)
+val in_place_map:
+  #a:Type0 ->
+  b: buffer a ->
+  l: UInt32.t{ UInt32.v l = Buffer.length b } ->
+  f:(a -> Tot a) ->
+  Stack unit
+    (requires (fun h -> live h b))
+    (ensures (fun h_1 r h_2 -> modifies_1 b h_1 h_2 /\ live h_2 b /\ live h_1 b
+      /\ (let s1 = as_seq h_1 b in
+         let s2 = as_seq h_2 b in
+         s2 == seq_map f s1) ))
+let in_place_map #a b l f =
+  let h0 = ST.get() in
+  let inv (h1: HS.mem) (i: nat): Type0 =
+    live h1 b /\ modifies_1 b h0 h1 /\ i <= UInt32.v l
+    /\ (forall (j:nat). {:pattern (get h1 b j)} (j >= i /\ j < UInt32.v l) ==> get h1 b j == get h0 b j)
+    /\ (forall (j:nat). {:pattern (get h1 b j)} j < i ==> get h1 b j == f (get h0 b j))
+  in
+  let f' (i:UInt32.t{ UInt32.( 0 <= v i /\ v i < v l ) }): Stack unit
+    (requires (fun h -> inv h (UInt32.v i)))
+    (ensures (fun h_1 _ h_2 -> UInt32.(inv h_2 (v i + 1))))
+  =
+    b.(i) <- f (b.(i))
+  in
+  for 0ul l inv f';
+  let h1 = ST.get() in
+  Seq.lemma_eq_intro (as_seq h1 b) (seq_map f (as_seq h0 b))
+
+
+(** Extracts as (destination buffer comes first):
+ * for (int i = 0; i < <l>; ++i)
+ *   in1[i] = <f>(in1[i], in2[i]);
+ *)
+val in_place_map2:
+  #a:Type0 -> #b:Type0 ->
+  in1: buffer a ->
+  in2: buffer b{disjoint in1 in2} ->
+  l: UInt32.t{ UInt32.v l = Buffer.length in1 /\ UInt32.v l = Buffer.length in2} ->
+  f:(a -> b -> Tot a) ->
+  Stack unit
+    (requires (fun h -> live h in1 /\ live h in2))
+    (ensures (fun h_1 r h_2 -> modifies_1 in1 h_1 h_2 /\ live h_2 in1 /\ live h_2 in2
+      /\ live h_1 in1 /\ live h_1 in2
+      /\ (let s1 = as_seq h_1 in1 in
+         let s2 = as_seq h_1 in2 in
+         let s = as_seq h_2 in1 in
+         s == seq_map2 f s1 s2) ))
+let in_place_map2 #a #b in1 in2 l f =
+  let h0 = ST.get() in
+  let inv (h1: HS.mem) (i: nat): Type0 =
+    live h1 in1 /\ live h1 in2 /\ modifies_1 in1 h0 h1 /\ i <= UInt32.v l
+    /\ (forall (j:nat). {:pattern (get h1 in1 j)} (j >= i /\ j < UInt32.v l) ==> get h1 in1 j == get h0 in1 j)
+    /\ (forall (j:nat). {:pattern (get h1 in1 j)} j < i ==> get h1 in1 j == f (get h0 in1 j) (get h0 in2 j))
+  in
+  let f' (i:UInt32.t{ UInt32.( 0 <= v i /\ v i < v l ) }): Stack unit
+    (requires (fun h -> inv h (UInt32.v i)))
+    (ensures (fun h_1 _ h_2 -> UInt32.(inv h_2 (v i + 1))))
+  =
+    in1.(i) <- f (in1.(i)) (in2.(i))
+  in
+  for 0ul l inv f';
+  let h1 = ST.get() in
+  Seq.lemma_eq_intro (as_seq h1 in1) (seq_map2 f (as_seq h0 in1) (as_seq h0 in2))
+
+
+#reset-options "--initial_fuel 2 --max_fuel 2 --z3rlimit 20"
+
+
+(* Repeating the same operation a number of times over a buffer ***************)
+
+val repeat_spec: #a:Type -> n:nat -> (f: a -> Tot a) -> a -> Tot a (decreases n)
+let rec repeat_spec #a n f x = if n = 0 then x else repeat_spec (n-1) f (f x)
+
+private
+val lemma_repeat: #a:Type -> n:nat{n > 0} -> f:( a -> Tot a) -> x:a -> Lemma
+  (repeat_spec n f x == f (repeat_spec (n-1) f x))
+let rec lemma_repeat #a n f x =
+  if n = 1 then ()
+  else lemma_repeat (n-1) f (f x)
+
+private
+val lemma_repeat_0: #a:Type -> n:nat{n = 0} -> f:( a -> Tot a) -> x:a -> Lemma
+  (repeat_spec n f x == x)
+let rec lemma_repeat_0 #a n f x = ()
+
+(** To be extracted as:
+ * for (int i = 0; i < n; ++i)
+ *   f(b[i]);
+ *)
+val repeat:
+  #a:Type0 ->
+  #len:nat ->
+  #f:(s:Seq.seq a{Seq.length s = len} -> Tot (s':Seq.seq a{Seq.length s' = Seq.length s})) ->
+  b: buffer a ->
+  l: UInt32.t{ UInt32.v l = Buffer.length b /\ UInt32.v l = len } ->
+  n:UInt32.t ->
+  f':(b:buffer a{length b = len} -> Stack unit
+                     (requires (fun h -> live h b))
+                     (ensures (fun h0 _ h1 -> live h0 b /\ live h1 b /\ modifies_1 b h0 h1
+                       /\ (let b0 = as_seq h0 b in
+                          let b1 = as_seq h1 b in
+                          b1 == f b0)))) ->
+  Stack unit
+    (requires (fun h -> live h b ))
+    (ensures (fun h_1 r h_2 -> modifies_1 b h_1 h_2 /\ live h_1 b /\ live h_2 b
+      /\ (let s = as_seq h_1 b in
+         let s' = as_seq h_2 b in
+         s' == repeat_spec (UInt32.v n) f s) ))
+let repeat #a #len #f b l max fc =
+  let h0 = ST.get() in
+  let inv (h1: HS.mem) (i: nat): Type0 =
+    live h1 b /\ modifies_1 b h0 h1 /\ i <= UInt32.v max
+    /\ as_seq h1 b == repeat_spec i f (as_seq h0 b)
+  in
+  let f' (i:UInt32.t{ UInt32.( 0 <= v i /\ v i < v max ) }): Stack unit
+    (requires (fun h -> inv h (UInt32.v i)))
+    (ensures (fun h_1 _ h_2 -> UInt32.(inv h_2 (v i + 1))))
+  =
+    fc b;
+    lemma_repeat (UInt32.v i + 1) f (as_seq h0 b)
+  in
+  lemma_repeat_0 0 f (as_seq h0 b);
+  for 0ul max inv f'
